$\vec{a}\neq 0$
$\vec{b} \neq 0$

$\angle(\vec{a},\vec{b})=\phi$ —  угол между векторами
$\angle(\vec{0}, \vec{a})=\frac{\pi}{2}$

$\vec{a}\perp \vec{b}$, если $\angle(\vec{a},\vec{b})=\frac{\pi}{2}$

**Ось** — прямая с заданным направлением.

![[vector_projection_p_planar.svg]]
$$
\text{При ПР}_{\vec{l}} \vec{AB} =
\left\{
\begin{array}{l} 
|\vec{A_{1}B_{1}}| \implies  \vec{A_{1}B_{1}} \upuparrows \vec{l} \\
-|\vec{A_{1}B_{1}}| \implies  \vec{A_{1}B_{1}} \uparrow\downarrow \vec{l} \\
0 , \text{если }  \vec{A_{1}B_{1}} = \vec{0} \implies  A_{1}=B_{1} \Longleftrightarrow \vec{AB}\perp \vec{l}
\end{array}
\right.
$$

## Опр4
Если:
- $\vec{e} \neq\vec{0}$
- $|\vec{e}|=1$
То:
- $\vec{e}$ —  орт

## Опр5

## Опр6
$\vec{a} \perp \vec{b}$ если $\angle(\vec{a}, \vec{b})=\frac{\pi}{2}$


## Св-ва проекции
1. $\boxed{Пр_{\vec{l}\ }\vec{b}=|\vec{b}|\cos \phi, \phi=\angle(\vec{b}, \vec{l})}$
   - Если $\vec{b} = \vec{0}$ это очевидно
   - Если $b\neq0$
		   - Если $\phi < \frac{\pi}{2}$
			   - $\cos \phi=\frac{{|\vec{A_{1}B_{1}}|}}{|\vec{a}|}\impliesпр_{\vec{l}}\vec{a}=|\vec{a}|\cos \phi$
		   - Если $\phi > \frac{\pi}{2}$
			   - $\cos \phi_{1}=-\cos \phi$
			   - $пр_{\vec{l}}\ \vec{a}=-|\vec{A_{1}B_{1}}|=|\vec{a}|\cos \phi$
	   
1.  $\boxed{пр_{\vec{l}\ }\lambda \vec{b}=\lambdaпр_{\vec{l}\ }\vec{b}}$
	   - $\vec{b} = \vec{0}, или \ \lambda=0$, то очевидно
	   - $\vec{b}\neq\vec{0}, \lambda\neq0$
	   - ---
	   - $\lambda >0$
			   - $\lambda \vec{a}\upuparrows\vec{a}$
			   - $пр_{\vec{l}}\lambda \vec{a}=|\lambda \vec{a}|\cos \angle(\lambda \vec{a};\vec{l})=\lambda|\vec{a}|\cos \angle(\lambda \vec{a};\vec{l})=$
			   - $=\lambda|\vec{a}|\cos \angle(\vec{a};\vec{l})=\lambdaпр_{\vec{l}} \ \vec{a}$
	   - ---
	   - $\lambda<0$
			   - $\lambda \vec{a}\uparrow\downarrow\vec{a}$
			   - $пр_{\vec{l}}\ \lambda \vec{a}=|\lambda \vec{a}|\cos \angle(\lambda\vec{a};\vec{l})=-\lambda|\vec{a}|\cos \angle(\lambda \vec{a};\vec{l})=$
			   - $\lambda |\vec{a}|\cos \angle(\vec{a};\vec{l})=\lambdaпр_{\vec{l}}\ \vec{a}$
		   - ---
2. $\boxed{пр_{\vec{l}\ }(\vec{a}+\vec{b})=пр_{\vec{l}\ }\vec{a}+пр_{\vec{l}\ }\vec{b}}$
   $\vec{c}=\vec{a}+\vec{b}$
	   - $пр_{\vec{l}}\ \vec{c}=-|\vec{OB_{1}}|$
	   - $пр_{\vec{l}}\ \vec{a} = |\vec{OA_{1}}|$
	   - $пр_{\vec{l}}\ \vec{b}=-|\vec{A_{1}B_{1}}|$
	   - $|\vec{A_{1}B_{1}}|=|\vec{OA_{1}}|+|\vec{OB_{1}}|$
![[triangle_vec_sum_projection.svg]]
### Проекция вектора на вектор
$b\neq0$
$пр_{\vec{b}}\ \vec{a}=пр_{\vec{l}}\ \vec{a}$ при $\vec{l}\upuparrows\vec{b}$