

$A\to A^{T}$ — транспонированая матрица
$A=(a_{ji})$
$A^{T}=(a_{ij})$

$\det A=\det A^{T}$

$\prod=a_{i_{1}k_{1}}a_{i_{2}k_{2}}\dots a_{i_{n}k_{n}}$ входит в $\det A$
в $\det A$ $\mathrm{sgn}\prod=(-1)^{t(p(i))+t(p(k))}$ входит в $\det A^{T}$

### Свво1

Если в определителе поменять местами любые две строки, то его знак изменится.

$A=\begin{pmatrix} \vec{a_{1}} \\ \vec{a_{k}}  \\ \vec{a_{l}}  \\ \vec{a_{n}}\end{pmatrix}$ $B=\begin{pmatrix} \vec{b_{1}} \\ \vec{b_{k}}  \\ \vec{b_{l}}  \\ \vec{b_{n}}\end{pmatrix}$

$\vec{a_{1}}=\vec{b_{1}}$
$\vec{b_{k}}=\vec{a}_{l}$
$\vec{b}_{k}=\vec{a}_{l}$
$\vec{b_{l}}=\vec{a_{k}}$
$\vec{b}_{k}=\vec{a}_{n}$

$\prod=a_{1j_{1}}\dots a_{kj_{k}}\dots a_{lj_{l}}\dots a_{nj_{n}}=b_{1j_{1}}\dots b_{lj_{k}}\dots b_{kj_{l}}\dots b_{nj_{n}}=t(p(1,\dots l\dots k\dots n))=(-1)^{t(p(j))}$

### Свво4

$|A|=\begin{pmatrix}\vec{a}_{1} \\ \vec{a}_{k}  \\ \dots\\ \vec{a}_{n}\end{pmatrix}=\lambda_{1}\cancelto{ \ \Delta_{1} }{ \begin{pmatrix}\vec{a}_{1} \\ \vec{b}_{k} \\ \dots \\ \vec{a}_{n}\end{pmatrix} }+\dots+\lambda_{s}\cancelto{ \ \Delta_{s} }{ \begin{pmatrix}\vec{a}_{1} \\ \vec{b}_{k} \\ \dots \\ \vec{a}_{n}\end{pmatrix} }$

$|A|=\sum_{p(j)}(-1)^{t(p(j))}a_{1j1}\dots a_{kjk}\dots a_{njn}=\sum_{p(j)}(-1)^{t(p(j))}a_{1j 1}\dots(\lambda_{1}b^{(1)}_{kjk}+\dots+\lambda_{s}b_{k}^{(s)})=a_{njn}=$
$=a_{1j 1}\dots b^{(1)}_{kjk}\dots a_{njn}+\dots+\lambda_{s}\sum_{p(j)}(-1)^{t(p(j))}a_{1jn}\dots b^{(s)}_{kjk}\dots a_{njn}=\lambda_{1}\Delta_{1}+\dots+\lambda _s\Delta_{s}$

### Свво5

$\det \begin{pmatrix}\vec{a}_{1} \\ \lambda\vec{a}_{k} \\ \vec{a}_{n}\end{pmatrix}=\lambda \det\begin{pmatrix}\vec{a}_{1} \\ \vec{a}_{k} \\ \vec{a}_{n}\end{pmatrix}$

### Свво6

$\det \begin{pmatrix}\vec{a}_{1} \\ \vec{0} \\ \vec{a}_{n}\end{pmatrix}=\det \begin{pmatrix}\vec{a}_{1} \\ 0\cdot\vec{0} \\\vec{a}_{n}\end{pmatrix}=0\cdot \det \begin{pmatrix}\vec{a}_{1} \\ \vec{0} \\ \vec{a}_{n}\end{pmatrix}=0$

### Свво7

!!8-10
