$|r_{1}-r_{2}|=2a\ (1)$
$\rho(F_{1},F_{2})=2c;\ c>a$
$c$ — фокусное расстояние

$\left|\sqrt{ (x_+c)^{2} + y^{2} }-\sqrt{ (x-c)^{2} + y^{2} }\right|=2a\ (2)$
$x^{2}\cancel{ +2xc+ }y^{2}+x^{2}\cancel{ -2cx }+c^{2}+y^{2}-2\sqrt{ (x^{2}+c^{2}+y^{2}+2cx)(x^{2}+c^{2}+y^{2}-2cx) }=4a^{2}$

$2(x^{2}+y^{2}+c^{2})-2\sqrt{ (x^{2}+y^{2}+c^{2})^{2}-4c^{2}x^{2} }=4a^{2}$
$t^{2}:=x^{2}+y^{2}+c^{2}$
$t^{2}-2a^{2}=\sqrt{ t^{4}-4c^{2}x^{2} }$
$\cancel{ t^{4} }-4t^{2}a^{2}+4a^{4}=\cancel{ t^{4} }-4c^{2}x^{2}$
$c^{2}x^{2}-(x^{2}+c^{2}+y^{2})a^{2}=-a^{4}$
$c^{2}x^{2}-a^{2}x^{2}-y^{2}a^{2}=c^{2}a^{2}-a^{4}$
$(c^{2}-a^{2})x^{2}-y^{2}a^{2}=a^{2}(c^{2}-a^{2})$

\*) $b^{2}:=(c^{2}-a^{2})$ т.к. $c>a$
$b^{2}x^{2}-a^{2}y^{2}=a^{2}b^{2}$

$\boxed{\frac{x^{2}}{a^{2}}-\frac{y^{2}}{b^{2}}=1}\ (3)$ — каноническое уравнение гиперболы

\*) $y^{2}=\left( \frac{x^{2}}{a^{2}}-1 \right)b^{2}$
$r_{1}=\sqrt{ (x+c)^{2}+y^{2} }=\sqrt{ x^{2}+2cx+c^{2}+ \frac{x^{2}}{a^{2}}(c^{2}-a^{2})+a^{2}-c^{2} }=\sqrt{ \cancel{ x^{2} }+2cx\cancel{ +c^{2} }+\frac{x^{2}}{a^{2}}\cdot c^{2}\cancel{ -x^{2} }+a^{2}\cancel{ -c^{2} } }=\sqrt{ a^{2}+2a \frac{x}{a}c+\left( \frac{x}{a}c \right)^{2} }=\left|a+\frac{c}{ax}\right|$
т.к. 
- $x>0$
- $\frac{x}{a}>1$
- $x>a$
- $c>a$

$r_{1}=\left|a+\frac{c}{a}x\right|=a+\frac{c}{a}x$
$r_{2}=\left| a-\frac{c}{a}x\right|=-a+\frac{c}{a}x$

$|r_{1}-r_{2}|=\left|-a-\cancel{ \frac{c}{a}x }-\cancel{ a+\frac{c}{a}x }\right|=|-2a|=2a$

$\boxed{\frac{x^{2}}{a^{2}}-\frac{y^{2}}{b^{2}}=1\longleftrightarrow\frac{y^{2}}{b^{2}}-\frac{x^{2}}{a^{2}}=-1}\ (3')$

Асимптоты:
$\hat{y_{1}}=\frac{b}{a}x$
$\hat{y_{2}}=-\frac{b}{a}x$

$$
\left[
\begin{array}{l}

x>a,x\to+\infty \\
\hat{y_{1}}=\dfrac{b}{a}x
\end{array}
\right.
$$
$y>0$

$\left|y(x)-\frac{b}{a}x\right|\to0,x\to+\infty$
$y=\sqrt{ \left( \frac{x^{2}}{a^{2}}-1 \right)b^{2} }$


