
$f^{(n)}(x):=(f^{(n-1)}(x))'$

$f^{(0)}(x):=f(x)$

### Теор. Правило Лейбница

$(uv)^{(n)}=\sum_{k=0}^{n}C_{n}^{k}u^{(k)}v^{(n-k)}$

### Докво (ММИ)

1. $n=1$
   $(uv)'=u'v+uv'=\sum_{k=0}^{1}C_{n}^{k}u^{(k)}v^{(1-k)}$
2. $m\implies m+1$
   $(uv)^{(m+1)}=((uv)^{(m)})'=\left( \sum_{k=0}^{m}C_{n}^{k}u^{(k)}v^{(m-k)} \right)=\sum_{k=0}^{m}C_{m}^{k}(u^{(k+1)}v^{(m-k)}+u^{(k)}v^{(m+1-k)})$
   $=C_{m}^{0}u^{(0)}v^{(m+1)}+\sum_{k=1}^{m}C_{m}^{k}u^{(k)}v^{(m+1-k)}+\sum_{k=0}^{m-1}C_{m}^{k}u^{(k+1)}v^{(m-k)}+C_{m}^{m}u^{(m+1)}v^{(0)}=$
   $j:=k+1$
   $=C_{m+1}^{0}u^{(0)}v^{(m+1)}+\sum_{k=1}^{m}C_{n}^{k}u^{(k)}v^{(m+1-t)}+\sum_{j=1}^{m}C_{m}^{j-1}u^{(j)}v^{(m+1-j)}+C_{m+1}^{m+1}u^{(m+1)}v^{(0)}=$
   $=C_{m+1}^{0}n^{(0)}v^{(m+1)}\sum_{k=1}^{m}(C_{m}^{k}+C_{m}^{k-1})u^{(k)}v^{(m+1-k)}+C_{m+1}^{m+1}u^{(m+1)}v^{(0)}=$ 
   $=$!!